template-coq/src/ast_quoter.ml
@@ -52,7 +52,7 @@ struct
   type quoted_constant_body = constant_body
   type quoted_global_decl = global_decl
   type quoted_global_declarations = global_declarations
-  type quoted_retroknowledge = Retroknowledge.t
+  type quoted_retroknowledge = Environment.Retroknowledge.t
   type quoted_global_env = global_env
   type quoted_program = program
 
@@ -327,7 +327,8 @@ struct
       retro_float64 : quoted_kernel_name option }
 
   let quote_retroknowledge r = 
-    { Retroknowledge.retro_int63 = r.retro_int63; Retroknowledge.retro_float64 = r.retro_float64 }
+    { Environment.Retroknowledge.retro_int63 = r.retro_int63; 
+      Environment.Retroknowledge.retro_float64 = r.retro_float64 }
 
   let mk_global_env universes declarations retroknowledge = { universes; declarations; retroknowledge }
   let mk_program decls tm = (decls, tm)
