pcuic/theories/Syntax/PCUICInduction.v
@@ -19,8 +19,6 @@ Import PCUICEnvTyping.
   Allows to get the right induction principle on lists of terms appearing
   in the term syntax (in evar, applications, branches of cases and (co-)fixpoints. *)
 
-Notation prim_ind P p := (P (tPrim p)).
-
 (** Custom induction principle on syntax, dealing with the various lists appearing in terms. *)
 
 Lemma term_forall_list_ind :
@@ -43,7 +41,7 @@ Lemma term_forall_list_ind :
     (forall (s : projection) (t : term), P t -> P (tProj s t)) ->
     (forall (m : mfixpoint term) (n : nat), tFixProp P P m -> P (tFix m n)) ->
     (forall (m : mfixpoint term) (n : nat), tFixProp P P m -> P (tCoFix m n)) ->
-    (forall p, prim_ind P p) ->
+    (forall p, P (tPrim p)) ->
     forall t : term, P t.
 Proof.
   intros until t. revert t.
@@ -261,7 +259,7 @@ Lemma term_forall_mkApps_ind :
     (forall (s : projection) (t : term), P t -> P (tProj s t)) ->
     (forall (m : mfixpoint term) (n : nat), tFixProp P P m -> P (tFix m n)) ->
     (forall (m : mfixpoint term) (n : nat), tFixProp P P m -> P (tCoFix m n)) ->
-    (forall i, prim_ind P i) ->
+    (forall i, P (tPrim i)) ->
     forall t : term, P t.
 Proof.
   intros until t.
